strandlib.v
@@ -1,0 +1,195 @@
+Require Import Logic List ListSet Arith Peano_dec Omega Ensembles.
+Require Import Coq.Sets.Constructive_sets.
+Require Import Finite_sets_facts Finite_sets Relation_Definitions.
+Require Import Relation_Operators.
+Require Import strictorder set_rep_equiv util.
+Require Import finite_set_builder.
+Require Import LibTactics.
+
+Require Import strandspace.
+
+Open Scope list_scope.
+Import ListNotations.
+Open Scope ss_scope.
+
+Hint Resolve Coq.Sets.Constructive_sets.Add_not_Empty Noone_in_empty.
+Hint Unfold Origin.
+
+Lemma origin_tx : forall n t,
+Origin t n ->
+is_tx n.
+Proof. unfold Origin. iauto. Qed.
+Hint Resolve origin_tx.
+Lemma origin_st : forall n t,
+Origin t n -> t <st msg n. 
+Proof. unfold Origin. iauto. Qed.
+Hint Resolve origin_st.
+Lemma origin_nopred_st : forall n t,
+Origin t n ->
+forall n', n' << n -> ~ t <st msg n'.
+Proof. unfold Origin. iauto. Qed.
+Hint Resolve origin_nopred_st.
+
+Lemma particular_min_smsg:
+  forall {min actual_content},
+    ((strand min) = [actual_content]) ->
+    smsg min = actual_content.
+Proof.
+  intros min actual_content seq.
+  assert (length (strand min) = 1) as len. rewrite seq. auto.
+  assert ((index min) = 0) as imin. 
+  remember (index_len_node min). omega. 
+  assert (nth_error (strand min) (index min) = Some (smsg min)) as ntheq. 
+  apply node_indexing_equiv.
+  rewrite seq in ntheq. rewrite imin in ntheq. simpl in ntheq.
+  inversion ntheq as [msmsg].
+  auto.
+Qed.
+Lemma particular_min_msg:
+  forall {min actual_content},
+    ((strand min) = [actual_content]) ->
+    msg min = smsg_msg actual_content.
+Proof.
+  intros min actual_content seq.
+  unfold msg.
+  erewrite particular_min_smsg.
+  tauto. auto.
+Qed.
+Lemma key_st_text_false : forall k t,
+(#k) <st (!t) -> False.
+Proof. intros. inversion H. Qed.
+Hint Resolve key_st_text_false.
+
+Lemma tx_rx_false : forall n,
+is_tx n -> is_rx n -> False.
+Proof. intros. inversion H. inversion H0. rewrite H2 in *. inversion H1. Qed.
+Hint Resolve tx_rx_false.
+Hint Unfold is_tx is_rx.
+
+Lemma node_strand_3height_opts : forall (n:Node) (sm1 sm2 sm3:SMsg),
+(strand n) = [sm1; sm2; sm3] ->
+(smsg n) = sm1 \/ (smsg n) = sm2 \/ (smsg n) = sm3.
+Proof. 
+  intros.
+  assert ((index n) = 0 \/ (index n) = 1 \/ (index n) = 2 \/ (index n) > 2). omega. 
+  destruct H0; forwards*: (node_indexing_equiv n).
+  rewrite H0 in *. rewrite H in *. simpl in *; inversion H1.
+  left. auto. destruct H0.
+  rewrite H0 in *. rewrite H in *. simpl in *; inversion H1.
+  right. left. auto. destruct H0.
+  rewrite H0 in *. rewrite H in *. simpl in *; inversion H1.
+  right. right. auto.
+  destruct n. simpl in *. assert (length (fst x) = 3). rewrite H. 
+  simpl. reflexivity. omega.
+Qed.
+Hint Resolve node_strand_3height_opts.
+
+Lemma nth_error_some_In {X:Type}: forall l i (x:X),
+nth_error l i = Some x ->
+List.In x l.
+Proof.
+  intros l. induction l.
+  intros i x nth. destruct i. simpl in nth; inversion nth.
+  simpl in nth; inversion nth.
+  intros i x nth.
+  destruct i. simpl in nth. inversion nth. left. reflexivity.
+  simpl in nth. right. eapply IHl. exact nth.
+Qed.
+Hint Resolve nth_error_some_In.
+
+Lemma node_smsg_in_strand : forall n s,
+(strand n) = s ->
+List.In (smsg n) s.
+Proof.
+  intros.
+  forwards*: (node_indexing_equiv n).
+  eapply nth_error_some_In. subst. exact H0.
+Qed.  
+Hint Resolve node_smsg_in_strand.
+
+Lemma node_hd_or_rest : forall n h rest,
+(strand n) = h :: rest ->
+(smsg n) = h \/ List.In (smsg n) rest.  
+Proof.
+  intros n h rest seq. 
+  forwards*: (node_smsg_in_strand n (h :: rest)).
+Qed.
+Hint Resolve node_hd_or_rest.
+
+Lemma hd_pred_all : forall n n',
+(strand n) = (strand n') ->
+(index n) = 0 ->
+(index n') > 0 ->
+n << n'.
+Proof.
+  intros n n' streq ni n'i.
+  apply spath_imp_sspath.
+  apply spath_from_props. omega. assumption.
+Qed.
+Hint Resolve hd_pred_all.
+
+Lemma no_origin_after_rx : forall n g rest,
+(strand n) = (-g) :: rest ->
+~Origin g n.
+Proof.
+  intros n g rest streq orig.
+  forwards*: node_hd_or_rest.
+  destruct orig as [Htx [Hst Hnopred]].
+  destruct H. forwards*: tx_rx_false.
+  assert (exists n0, (index n0) = 0 /\ (strand n0) = (strand n)).
+  eexists (exist _ ((strand n), 0) _). simpl. auto.
+  destruct H0 as [n0 [n0s n0i]].
+  assert (n0 << n). apply hd_pred_all; auto.
+  (* BOOKMARK *)
+  forwards*: hd_pred_all.
+  Admitted.
+
+
+
+Lemma origin_imp_st_strand : forall t x s,
+Origin t x ->
+strand x = s ->
+st_on_strand t s = true.
+Proof.
+  Admitted.
+Hint Resolve origin_imp_st_strand.
+
+Lemma equiv_disjunct : forall p,
+p \/ p -> p.
+Proof. intros. iauto. Qed.
+
+Lemma strand_prev_imp_pred : forall f n x xs,
+strand n = f ++ x :: xs ->
+smsg n <> x ->
+exists n', n' << n /\ smsg n' = x.
+Proof.
+  Admitted.
+Hint Resolve strand_prev_imp_pred.
+
+Lemma no_st_l_r : forall l r t,
+~ t <st l ->
+~ t <st r ->
+t <> (l * r) ->
+~ t <st (l * r).
+Proof.
+  intros l r t notl notr neq contra.
+  inversion contra; subst; auto.
+Qed.
+Hint Resolve no_st_l_r.
+
+Lemma key_st_key : forall (k k' : Key),
+(#k) <st (#k') -> k = k'.
+Proof. 
+  intros. inversion H; auto.
+Qed.  
+Hint Resolve key_st_key.
+
+Lemma no_encr_st : forall a b k,
+~ a <st b ->
+a <> {b}^[k] ->
+~ a <st {b}^[k].
+Proof.
+  intros a b k nost neq contra. 
+  inversion contra; eauto. 
+Qed.
+Hint Resolve no_encr_st.
