strandspaceNSL.v
@@ -1,0 +1,63 @@
+
+Require Import Logic List ListSet Arith Peano_dec Omega Ensembles.
+Require Import Finite_sets_facts Finite_sets Relation_Definitions.
+Require Import Relation_Operators.
+Require Import strictorder set_rep_equiv util.
+Require Import finite_set_builder.
+
+Require Import strandspace.
+
+Section NSLSpace.
+
+Open Scope list_scope.
+Import ListNotations.
+Open Scope ss_scope.
+
+Hypothesis PModel : PenetratorModel = DolevYao.
+Variable A B Na Nb : Text.
+  Hypothesis neqANa : A <> Na.
+  Hypothesis neqANb : A <> Nb.
+  Hypothesis neqBNa : B <> Na.
+  Hypothesis neqBNb : B <> Nb.
+Variable Ka Kb : Key.
+  Hypothesis keyinj : Ka = Kb -> A = B.
+
+Hypothesis NSLProtocol : 
+  Protocol = [[(+ {(!Na) * (!A)}^[Kb]) ; 
+               (- {(!Na) * (!Nb) * (!B)}^[Ka]) ;
+               (+ {(!Nb)}^[Kb])] ; 
+              [(- {(!Na) * (!A)}^[Kb]) ; 
+               (+ {(!Na) * (!Nb) * (!B)}^[Ka]) ;
+               (- {(!Nb)}^[Kb])]].
+
+(* Proposition 5.2
+   Suppose:
+   1) The SS is an NSL space, C is a bundle in it,
+      and s is a responder strand
+      Resp[A, B, Na, Nb] with C-height 3. 
+   2) inv(Ka) is not in Kp
+   3) Na <> Nb and Nb is uniquely originating in the space. 
+   THEN
+    C contains an initiator's strand t (Init[A, B, Na, Nb] with 
+    C-height 3. *)
+Definition s : Strand :=  [(- {(!Na) * (!A)}^[Kb]) ; 
+               (+ {(!Na) * (!Nb) * (!B)}^[Ka]) ;
+               (- {(!Nb)}^[Kb])].
+
+Lemma s_regular : RegularStrand s.
+Proof.
+  unfold RegularStrand. rewrite NSLProtocol.
+  unfold s. right. left. reflexivity.
+Qed.
+(*
+Lemma ex_n0 : 
+  exists n0, (strand n0) = s /\ (index n0) = 2.
+Proof.
+  *)
+
+(* Lemma 5.3 Nb originates at n0 *)
+
+
+
+
+End NSLSpace.
