strandspacegeneric.v
@@ -1,11 +1,13 @@
 
 Require Import Logic List ListSet Arith Peano_dec Omega Ensembles.
+Require Import Coq.Sets.Constructive_sets.
 Require Import Finite_sets_facts Finite_sets Relation_Definitions.
 Require Import Relation_Operators.
 Require Import strictorder set_rep_equiv util.
 Require Import finite_set_builder.
+Require Import LibTactics.
 
-Require Import strandspace.
+Require Import strandspace strandlib.
 
 Section SimpleSpaces.
 
@@ -14,6 +16,7 @@ Hypothesis PModel : PenetratorModel = DolevYao.
 Open Scope list_scope.
 Import ListNotations.
 Open Scope ss_scope.
+
 
 (* Proposition 3.3 
    "Let C be a bundle, and let k be a Key s.t. ~ k in Kp,
@@ -41,288 +44,107 @@ Proof.
               Pdec
               N 
               finN) 
-    as [N' [inclN' N'memP]].
-  assert (Finite Node N') as finN'. eapply Finite_downward_closed.
-    exact finN. exact inclN'.
-  destruct finN' as [| N' fin x].
-  Case "Empty_set".
-    assert (In Node (Empty_set Node) n) as  contra.
-      apply N'memP. split. exact nInN. exact st.
-    inversion contra.
+    as [N' [inclN' [N'memP PmemN']]].
+  forwards*: (Finite_downward_closed Node N finN N').
+  destruct H as [| N' fin x].
+  Case "Empty_set". 
+    forwards: PmemN'. eauto. contradiction.
   Case "non-empty".
-    assert (exists min, set_minimal (Add Node N' x) min) as exmin.
-      eapply (bundle_subset_minimal B). rewrite <- NB. exact inclN'.
-      intros contra. apply Add_not_Empty in contra. contradiction.
-    destruct exmin as [min minP].
-    assert (Origin (#k) min) as minorg.
-      eapply (min_origin B (Add Node N' x)). split.
-      intros [mIn mst].
-      apply N'memP. split. rewrite NB. exact mIn. exact mst.
-      intros mIn. split.
-      apply inclN' in mIn. rewrite <- NB. exact mIn.
-      apply N'memP in mIn. destruct mIn; auto. exact minP.
-    destruct (align_dec (strand min)) as [reg | pen].
-    eapply noOrigin. exact minorg. exact reg.
-    destruct minorg as [istx [minst minpred]].
-    assert (DolevYao (strand min)) as dymin.
-    rewrite <- PModel. apply penetrator_behavior. exact pen.
-    inversion dymin as 
-      [s t tunk seq minstrand | 
-       s g seq minstrand |
-       s g seq minstrand |
-       s g h seq minstrand |
-       s g h seq minstrand |
-       s k' kunk seq minstrand |
-       s h k' seq minstrand |
-      s h k' k'' inv seq minstrand]. 
+    edestruct (bundle_subset_minimal B) as [min Hmin]. 
+      subst N. eauto. auto.
+    forwards: (min_origin B (Add Node N' x)). subst N. eauto. subst N. eauto.
+      eauto.
+    forwards*: origin_tx. forwards*: origin_st.
+    forwards*: (noOrigin). forwards*: (penetrator_behaviour).
+    rewrite PModel in *.
+    (* Case analysis on DolevYao variants *)
+    inversion H4 as 
+        [s t tunk seq minstrand | 
+         s g seq minstrand |
+         s g seq minstrand |
+         s g h seq minstrand |
+         s g h seq minstrand |
+         s k' kunk seq minstrand |
+         s h k' seq minstrand |
+         s h k' k'' inv seq minstrand]. 
     SCase "M".
-      assert (length (strand min) = 1) as len. rewrite seq. auto.
-      assert ((index min) = 0) as imin. 
-        remember (index_len_node min). omega. 
-      assert (nth_error (strand min) (index min) = Some (smsg min)) as ntheq. 
-      apply node_indexing_equiv. 
-      rewrite seq in ntheq. rewrite imin in ntheq. simpl in ntheq.
-      inversion ntheq as [msmsg]. 
-      assert (msg min = (!t)) as minmsg.
-      apply node_smsg_msg_tx; auto. rewrite minmsg in minst. 
-      inversion minst.
+      rewrite (particular_min_msg seq) in *. eauto.
     SCase "F".
-      assert (length (strand min) = 1) as len. rewrite seq. auto.
-      assert ((index min) = 0) as imin. remember (index_len_node min); omega.
-      assert (nth_error (strand min) (index min) = Some (smsg min)) as ntheq. 
-      apply node_indexing_equiv. 
-      rewrite seq in ntheq. rewrite imin in ntheq. simpl in ntheq.
-      destruct istx as [t mmsg]. rewrite mmsg in ntheq.
-      inversion ntheq.
+      forwards*: (tx_rx_false).
+      forwards*: (particular_min_smsg seq).
     SCase "T".
-      assert (length (strand min) = 3) as len. rewrite seq. auto.
-      assert ((index min) = 0 
-              \/ (index min) = 1 
-              \/ (index min) = 2) as imin. remember (index_len_node min); omega.
-      assert (nth_error (strand min) (index min) = Some (smsg min)) as ntheq. 
-      apply node_indexing_equiv. 
-      destruct imin as [imin | irest].
-      SSCase "index min = 0".
-        rewrite seq in ntheq. rewrite imin in ntheq. simpl in ntheq.
-        inversion ntheq as [mmsg]. destruct istx as [t mtx]. 
-        rewrite mtx in mmsg.
-        inversion mmsg.
-      destruct irest as [imin | imin].
-      SSCase "index min = 1".
-        rewrite seq in ntheq. rewrite imin in ntheq. simpl in ntheq.
-        inversion ntheq as [mintxmsg]. 
-        assert (msg min = g) as minmsg.
-        apply node_smsg_msg_tx; auto. rewrite minmsg in minst.
-        destruct (strand_node (strand min) 0) as [y [ys yi]].
-          rewrite seq. simpl; auto. 
-        assert (y << min) as ypremin. constructor.
-          constructor 2. constructor. rewrite ys. reflexivity.
-          omega.
-        apply minpred in ypremin.
-        assert (nth_error (strand min) (index y) = Some (smsg y)) as ntheq2.
-          rewrite <- ys.
-        apply node_indexing_equiv. rewrite seq in ntheq2. rewrite yi in ntheq2.
-        simpl in ntheq2. inversion ntheq2 as [rxmsg]. symmetry in rxmsg. 
-        eapply node_smsg_msg_rx in rxmsg. rewrite rxmsg in ypremin.
-        contradiction.
-      SSCase "index min = 2".
-        rewrite seq in ntheq. rewrite imin in ntheq. simpl in ntheq.
-        inversion ntheq as [mintx]. 
-        assert (msg min = g) as minmsg.
-        apply node_smsg_msg_tx; auto. rewrite minmsg in minst.
-        destruct (strand_node (strand min) 1) as [y [ys yi]].
-          rewrite seq. simpl; auto. 
-        assert (y << min) as ypremin. constructor.
-          constructor 2. constructor. rewrite ys. reflexivity.
-          omega.
-        apply minpred in ypremin.
-        assert (nth_error (strand min) (index y) = Some (smsg y)) as ntheq2.
-          rewrite <- ys.
-        apply node_indexing_equiv. rewrite seq in ntheq2. rewrite yi in ntheq2.
-        simpl in ntheq2. inversion ntheq2 as [rxmsg]. symmetry in rxmsg. 
-        eapply node_smsg_msg_tx in rxmsg. rewrite rxmsg in ypremin.
-        contradiction.      
+      forwards*: no_origin_after_rx.
+      edestruct (node_strand_3height_opts) as [rxg | txg]. eauto.
+      forwards*: tx_rx_false; forwards*: node_smsg_msg_tx.
+      forwards*: equiv_disjunct.
+      edestruct (strand_prev_imp_pred [] min (-g) [(+g); (+g)]) 
+        as [pred [plt psmsg]]. 
+        auto. eauto.
+      forwards*: origin_nopred_st. erewrite (node_smsg_msg_tx min g) in *.
+      rewrite (node_smsg_msg_rx pred g) in *. contradiction. 
+      auto. auto.
     SCase "C".
-      assert (length (strand min) = 3) as len. rewrite seq. auto.
-      assert ((index min) = 0 
-              \/ (index min) = 1 
-              \/ (index min) = 2) as imin. remember (index_len_node min); omega.
-      assert (nth_error (strand min) (index min) = Some (smsg min)) as ntheq. 
-      apply node_indexing_equiv. 
-      destruct imin as [imin | irest].
-      SSCase "index min = 0".
-        rewrite seq in ntheq. rewrite imin in ntheq. simpl in ntheq.
-        destruct istx as [t mtx]. rewrite mtx in ntheq.
-        inversion ntheq.
-      destruct irest as [imin | imin].
-      SSCase "index min = 1".
-        rewrite seq in ntheq. rewrite imin in ntheq. simpl in ntheq.
-        destruct istx as [t mtx]. rewrite mtx in ntheq.
-        inversion ntheq.
-      SSCase "index min = 2".
-        destruct (strand_node (strand min) 0) as [n0 [n0s n0i]].
-          rewrite seq. simpl; auto. 
-        destruct (strand_node (strand min) 1) as [n1 [n1s n1i]].
-          rewrite seq. simpl; auto. 
-        rewrite seq in ntheq. rewrite imin in ntheq. simpl in ntheq.
-        inversion ntheq as [mmsg]. symmetry in mmsg. 
-        apply node_smsg_msg_tx in mmsg. rewrite mmsg in minst.
-        inversion minst as [m | m l r Hst | m l r Hst | m1 m2 k1 Hst]; subst.
-        SSSCase "#k <st g".
-          assert (n0 << min) as n0pred. econstructor 2. constructor. 
-            constructor 2. constructor. rewrite n0s. symmetry in n1s. 
-            exact n1s. omega. constructor. constructor 2. constructor. 
-            exact n1s. omega.
-          apply minpred in n0pred. 
-          assert (nth_error (strand n0) (index n0) = Some (smsg n0)) as ntheq2. 
-            apply node_indexing_equiv.
-          rewrite n0i in ntheq2. rewrite n0s in ntheq2. rewrite seq in ntheq2.
-          simpl in ntheq2. inversion ntheq2 as [rxmsg]. symmetry in rxmsg.
-          apply node_smsg_msg_rx in rxmsg. rewrite rxmsg in n0pred.
-          contradiction.
-        SSSCase "#k <st h".
-          assert (n1 << min) as n1pred. econstructor. constructor 2. 
-            constructor. auto. omega.
-          apply minpred in n1pred.
-          assert (nth_error (strand n1) (index n1) = Some (smsg n1)) as ntheq2. 
-            apply node_indexing_equiv.
-          rewrite n1s in ntheq2. rewrite n1i in ntheq2. rewrite seq in ntheq2.
-          simpl in ntheq2. inversion ntheq2 as [rxmsg]. symmetry in rxmsg.
-          apply node_smsg_msg_rx in rxmsg.
-          rewrite rxmsg in n1pred. contradiction.
+      forwards*: no_origin_after_rx.
+      edestruct (node_strand_3height_opts) as [rxg | [rxh | txgh]]. eauto.
+      forwards*: tx_rx_false; forwards*: node_smsg_msg_tx.
+      forwards*: tx_rx_false; forwards*: node_smsg_msg_tx.
+      edestruct (strand_prev_imp_pred [] min (-g) [(-h); (+g * h)]) 
+        as [pred [plt psmsg]]. 
+        simpl. auto. eauto.
+      forwards*: (origin_nopred_st). 
+      edestruct (strand_prev_imp_pred [(-g)] min (-h) [(+g * h)]) 
+        as [pred2 [p2lt p2smsg]]. simpl. auto. eauto.
+      forwards*: (origin_nopred_st). 
+      rewrite (node_smsg_msg_tx min (g * h)) in *.
+      rewrite (node_smsg_msg_rx pred g) in *.
+      rewrite (node_smsg_msg_rx pred2 h) in *.
+      apply (no_st_l_r g h (#k)); auto. intros contra. inversion contra.
+      auto. auto. auto.
     SCase "S".
-      assert (length (strand min) = 3) as len. rewrite seq. auto.
-      assert ((index min) = 0 
-              \/ (index min) = 1 
-              \/ (index min) = 2) as imin. remember (index_len_node min); omega.
-      assert (nth_error (strand min) (index min) = Some (smsg min)) as ntheq. 
-      apply node_indexing_equiv. 
-      destruct imin as [imin | irest].
-      SSCase "index min = 0".
-        rewrite seq in ntheq. rewrite imin in ntheq. simpl in ntheq.
-        destruct istx as [t mtx]. rewrite mtx in ntheq.
-        inversion ntheq.
-      destruct irest as [imin | imin].
-      SSCase "index min = 1".
-        rewrite seq in ntheq. rewrite imin in ntheq. simpl in ntheq.
-        destruct (strand_node (strand min) 0) as [n0 [n0s n0i]].
-          rewrite seq. simpl; auto. 
-        assert (n0 << min) as n0pred. econstructor. constructor 2. 
-          constructor. auto. omega.
-        apply minpred in n0pred.
-        assert (nth_error (strand n0) (index n0) = Some (smsg n0)) as ntheq2.  
-          apply node_indexing_equiv.
-        rewrite n0s in ntheq2. rewrite n0i in ntheq2. rewrite seq in ntheq2.
-        simpl in ntheq2. inversion ntheq2 as [mrx]. symmetry in mrx.
-        apply node_smsg_msg_rx in mrx. rewrite mrx in n0pred.
-        assert (nth_error (strand min) (index min) = Some (smsg min)) as ntheq3. 
-          apply node_indexing_equiv.
-         rewrite seq in ntheq3. rewrite imin in ntheq3. simpl in ntheq3.
-         inversion ntheq3 as [mmsg]. symmetry in mmsg. 
-         apply node_smsg_msg_tx in mmsg.
-         rewrite mmsg in minst.
-         apply n0pred. constructor. exact minst.
-      SSCase "index min = 2".
-        rewrite imin in ntheq. rewrite seq in ntheq. simpl in ntheq.
-        destruct (strand_node (strand min) 0) as [n0 [n0s n0i]].
-          rewrite seq. simpl; auto. 
-        destruct (strand_node (strand min) 1) as [n1 [n1s n1i]].
-          rewrite seq. simpl; auto. 
-        assert (n0 << min) as n0pred. apply (t_trans Node SSEdge n0 n1 min). 
-          constructor. constructor 2. constructor. rewrite n0s. 
-          auto. omega. constructor. constructor 2. constructor.
-          exact n1s. omega.
-        apply minpred in n0pred.
-        assert (nth_error (strand n0) (index n0) = Some (smsg n0)) as ntheq2. 
-          apply node_indexing_equiv.
-        rewrite n0s in ntheq2. rewrite n0i in ntheq2. rewrite seq in ntheq2.
-        simpl in ntheq2. inversion ntheq2 as [mrx]. symmetry in mrx.
-        apply node_smsg_msg_rx in mrx. rewrite mrx in n0pred.
-        assert (nth_error (strand min) (index min) = Some (smsg min)) as ntheq3. 
-          apply node_indexing_equiv.
-         rewrite seq in ntheq3. rewrite imin in ntheq3. simpl in ntheq3.
-         inversion ntheq3 as [mtx]. symmetry in mtx. 
-         apply node_smsg_msg_tx in mtx.
-         rewrite mtx in minst.
-         apply n0pred. constructor 3. exact minst.
+      forwards*: no_origin_after_rx.
+      edestruct (node_strand_3height_opts) as [rxg | [rxh | txgh]]. eauto.
+      forwards*: tx_rx_false; forwards*: node_smsg_msg_tx.
+      edestruct (strand_prev_imp_pred [] min (-g * h) [(+g); (+h)]) 
+        as [pred [plt psmsg]]. 
+        simpl. auto. eauto.
+      forwards*: (origin_nopred_st). 
+      rewrite (node_smsg_msg_rx pred (g * h)) in *.
+      rewrite (node_smsg_msg_tx min (g)) in *. eauto. eauto.
+      auto.
+      edestruct (strand_prev_imp_pred [] min (-g * h) [(+g); (+h)]) 
+        as [pred [plt psmsg]]. 
+        simpl. auto. eauto.
+      forwards*: (origin_nopred_st). 
+      rewrite (node_smsg_msg_rx pred (g * h)) in *.
+      rewrite (node_smsg_msg_tx min (h)) in *. eauto. eauto.
+      auto.
     SCase "K".
-      destruct (eq_key_dec k k'); subst. contradiction.
-      assert (nth_error (strand min) (index min) = Some (smsg min)) as ntheq. 
-        apply node_indexing_equiv.
-      rewrite seq in ntheq. 
-      assert (length (strand min) = 1) as len. rewrite seq. auto.
-      assert ((index min) = 0)as imin. remember (index_len_node min); omega.
-      assert (nth_error (strand min) (index min) = Some (smsg min)) as ntheq2. 
-        apply node_indexing_equiv.
-      rewrite imin in ntheq2. rewrite seq in ntheq2. simpl in ntheq2.
-      inversion ntheq2 as [mtx]. symmetry in mtx. apply node_smsg_msg_tx in mtx.
-      rewrite mtx in minst.
-      inversion minst. contradiction.      
+      rewrite (particular_min_msg seq) in *. simpl in *.
+      forwards*: (key_st_key k k'). subst. contradiction.
     SCase "E".
-      assert (length (strand min) = 3) as len. rewrite seq. auto.
-      assert ((index min) = 0 
-              \/ (index min) = 1 
-              \/ (index min) = 2) as imin. remember (index_len_node min); omega.
-      assert (nth_error (strand min) (index min) = Some (smsg min)) as ntheq. 
-        apply node_indexing_equiv. 
-      destruct imin as [imin | irest].
-      SSCase "index min = 0".
-        rewrite imin in ntheq. rewrite seq in ntheq. simpl in ntheq.
-        inversion ntheq as [mrx]. destruct istx as [t mtx]. rewrite mtx in mrx.
-        inversion mrx.
-      destruct irest as [imin | imin].
-      SSCase "index min = 1".
-        rewrite imin in ntheq. rewrite seq in ntheq. simpl in ntheq.
-        inversion ntheq as [mrx]. destruct istx as [t mtx]. rewrite mtx in mrx.
-        inversion mrx.
-      SSCase "index min = 2".
-        rewrite imin in ntheq. rewrite seq in ntheq. simpl in ntheq.
-        inversion ntheq as [mtx]. symmetry in mtx. apply node_smsg_msg_tx in mtx.
-        rewrite mtx in minst.
-        inversion minst; subst.
-        destruct (strand_node (strand min) 1) as [n1 [n1s n1i]].
-          rewrite seq. simpl; auto.  
-        assert (n1 << min) as n1pre. constructor. constructor 2.
-          constructor. auto. omega.
-        apply minpred in n1pre.
-        assert (nth_error (strand n1) (index n1) = Some (smsg n1)) as ntheq2. 
-          apply node_indexing_equiv.        
-        rewrite n1i in ntheq2. rewrite seq in n1s. rewrite n1s in ntheq2. 
-        simpl in ntheq2. inversion ntheq2 as [mrx]. symmetry in mrx.
-        apply node_smsg_msg_rx in mrx. rewrite mrx in n1pre.
-        contradiction.
+      edestruct (node_strand_3height_opts) as [rxk | [rxh | txhk]]. eauto.
+      forwards*: tx_rx_false; forwards*: node_smsg_msg_tx.
+      forwards*: tx_rx_false; forwards*: node_smsg_msg_tx.
+      edestruct (strand_prev_imp_pred [(-(#k'))] min (-h) [(+{h}^[k'])]) 
+        as [pred [plt psmsg]]. simpl. auto. eauto.
+      forwards*: (origin_nopred_st). 
+      rewrite (node_smsg_msg_rx pred (h)) in *.
+      rewrite (node_smsg_msg_tx min {h}^[k']) in *.
+      forwards*: (no_encr_st (#k) h). intros neq.
+      inversion neq. eauto. eauto.
     SCase "D".
-      assert (length (strand min) = 3) as len. rewrite seq. auto.
-      assert ((index min) = 0 
-              \/ (index min) = 1 
-              \/ (index min) = 2) as imin. remember (index_len_node min); omega.
-      assert (nth_error (strand min) (index min) = Some (smsg min)) as ntheq. 
-        apply node_indexing_equiv. 
-      destruct imin as [imin | irest].
-      SSCase "index min = 0".
-        rewrite imin in ntheq. rewrite seq in ntheq. simpl in ntheq.
-        inversion ntheq as [mrx]. symmetry in mrx.
-        destruct istx as [t mtx]. rewrite mtx in mrx. inversion mrx.
-      destruct irest as [imin | imin].
-      SSCase "index min = 1".
-        rewrite imin in ntheq. rewrite seq in ntheq. simpl in ntheq.
-        inversion ntheq as [mrx]. symmetry in mrx.
-        destruct istx as [t mtx]. rewrite mtx in mrx. inversion mrx.
-      SSCase "index min = 2".
-        destruct (strand_node (strand min) 1) as [n1 [n1s n1i]].
-          rewrite seq. simpl; auto.  
-        assert (n1 << min) as n1pre. constructor. constructor 2.
-          constructor. auto. omega.
-        apply minpred in n1pre.
-        assert (nth_error (strand n1) (index n1) = Some (smsg n1)) as ntheq2. 
-          apply node_indexing_equiv.        
-        rewrite n1s in ntheq2. rewrite seq in ntheq2. rewrite n1i in ntheq2. 
-        simpl in ntheq2. inversion ntheq2 as [mrx]. symmetry in mrx.
-        apply node_smsg_msg_rx in mrx. rewrite mrx in n1pre.
-        rewrite imin in ntheq. rewrite seq in ntheq. simpl in ntheq.
-        inversion ntheq as [mtx]. symmetry in mtx.
-        apply node_smsg_msg_tx in mtx. rewrite mtx in minst.
-        apply n1pre. constructor. exact minst.
+      edestruct (node_strand_3height_opts) as [rxk | [rxh | txhk]]. eauto.
+      forwards*: tx_rx_false; forwards*: node_smsg_msg_tx.
+      forwards*: tx_rx_false; forwards*: node_smsg_msg_tx.
+      edestruct (strand_prev_imp_pred [(-(#k''))] 
+                                      min  
+                                      (-{h }^[ k']) 
+                                      [(+h)]) 
+        as [pred [plt psmsg]]. simpl. auto. eauto.
+      forwards*: (origin_nopred_st). 
+      rewrite (node_smsg_msg_rx pred ({h}^[k'])) in *.
+      rewrite (node_smsg_msg_tx min h) in *.
+      eauto. auto. auto.
 Qed.
 
 End SimpleSpaces.
